theories/heap_lang/lib/is_mon.v
@@ -1,0 +1,96 @@
+From iris.heap_lang Require Export heap.
+From iris.heap_lang Require notation.
+
+(* Minor annoyance: [solve_proper] can't handle our goals. *)
+Local Notation ext R := (pointwise_relation _ R).
+
+Ltac apply_eq :=
+  lazymatch goal with
+  | H : (eq ==> ext ?R)%signature ?f1 ?f2 |- ?R (?f1 ?x1 ?y1) (?f2 ?x1 ?y1)
+    => apply H
+  end.
+
+Ltac solve_proper_eq :=
+  preprocess_solve_proper;
+  repeat (f_equiv; try (eassumption || apply_eq)).
+
+(** * Value constructors *)
+
+Class constructor (A : Type) := Ctor {
+  ctor : A → val;
+  ctor_inj : Inj (=) (=) ctor
+}.
+
+Existing Instance ctor_inj.
+Arguments Ctor {_} _ _.
+
+Instance val_ctor : constructor val := Ctor id id_inj.
+
+Lemma locv_inj : Inj (=) (=) LocV. Proof. by move=>?? [] ->. Qed.
+Instance loc_constructor : constructor loc := Ctor LocV locv_inj.
+
+Coercion ctor : constructor >-> Funclass.
+
+(** * Reference monitors *)
+(**
+	The assertion [is_mon v Ψ1 Ψ2] means that [v] is a reference
+	monitor of "type" [Ψ1 → Ψ2] where [Ψ1] is a predicate on
+	inputs of type [A] and [Ψ2] relates inputs of type [A] to
+	outputs of type [B]. Both [A] and [B] must have [constructor]
+	instances.
+*)
+Section is_mon.
+  Context `{heapG Σ, fA : constructor A, fB : constructor B}.
+
+  Definition is_mon (v : val) (Ψ1 : A → iProp Σ)
+      (Ψ2 : A → B → iProp Σ) : iProp Σ :=
+    (∀ a, {{{ Ψ1 a }}} v (fA a) ?{{{ b, RET fB b; Ψ2 a b }}})%I.
+
+  Global Instance is_mon_persistent v Ψ1 Ψ2 :
+    PersistentP (is_mon v Ψ1 Ψ2).
+  Proof. apply _. Qed.
+
+  Global Instance is_mon_ne v n :
+    Proper (ext (dist n) ==> ((=) ==> ext (dist n)) ==> dist n) (is_mon v).
+  Proof. solve_proper_eq. Qed.
+
+  Global Instance is_mon_proper v :
+     Proper (ext (≡) ==> ((=) ==> ext (≡)) ==> (≡)) (is_mon v).
+  Proof. solve_proper_eq. Qed.
+End is_mon.
+Typeclasses Opaque is_mon.
+
+(** * Reference monitors *)
+(**
+	The assertion [is_monP v Ψ1 Ψ2] means that [v] is a reference
+	monitor of "type" [Ψ1 → Ψ2] where [Ψ1] and [Ψ2] are predicates
+	on inputs of type [A] and outputs of type [B], respectively.
+	Both [A] and [B] must have [constructor] instances.
+
+	This is just a special case of [is_mon] where [Ψ2] does not
+	depend on the input.
+*)
+Section is_monP.
+  Context `{heapG Σ, fA : constructor A, fB : constructor B}.
+
+  Definition is_monP (v : val) (Ψ1 : A → iProp Σ)
+      (Ψ2 : B → iProp Σ) : iProp Σ :=
+    (∀ a, {{{ Ψ1 a }}} v (fA a) ?{{{ b, RET fB b; Ψ2 b }}})%I.
+
+  Global Instance is_monP_persistent v Ψ1 Ψ2 :
+    PersistentP (is_monP v Ψ1 Ψ2).
+  Proof. apply _. Qed.
+
+  Global Instance is_monP_ne v n :
+     Proper (ext (dist n) ==> ext (dist n) ==> dist n) (is_monP v).
+  Proof. solve_proper. Qed.
+
+  Global Instance is_monP_proper v :
+     Proper (ext (≡) ==> ext (≡) ==> (≡)) (is_monP v).
+  Proof. solve_proper. Qed.
+
+  Lemma is_monP_rel v Ψ1 Ψ2 :
+    is_monP v Ψ1 Ψ2 ⊣⊢ is_mon v Ψ1 (λ _, Ψ2).
+  Proof. by []. Qed.
+End is_monP.
+Typeclasses Opaque is_monP.
